imp/definition/ImpPrelude.v
@@ -30,10 +30,13 @@ Global Program Instance EMSConfigImp: EMSConfig := {|
                 match rv↓ with
                 | Some (rv) =>
                   match rv with
-                  | Vint z => (0 <=? z)%Z && (z <? two_power_nat 32)%Z
-                  | _ => false
+                  | Vint z =>
+                    if (0 <=? z)%Z && (z <? two_power_nat 32)%Z
+                    then Some z↑
+                    else None
+                  | _ => None
                   end
-                | _ => false
+                | _ => None
                 end;
   initial_arg := ([]: list val)↑;
 |}
